backwards progress is still progress?

iocy/iocy_join.fst
@@ -360,13 +360,13 @@ let prog7 = Print 0 (fun () -> Fork (fun () -> Print 100 prog11) (fun () -> Prin
 // let _ = assert (theta' (prog12 ()) (fun r -> as_simpl_traces r == []) [] []) by (compute (); dump "foo")
 
 /// Quantified Linear Temporal logic on sets of finite traces [trs: list (list s)]
-///
+/// 
 /// We define the quantifier [quant] and ltl syntax [ltl_syntax].
 type quant =
 | Forall
 | Exists
 
-unopteq
+noeq
 type ltl_syntax (s:Type0) =
 | Eventually : ltl_syntax s -> ltl_syntax s
 | Always: ltl_syntax s -> ltl_syntax s
@@ -376,16 +376,14 @@ type ltl_syntax (s:Type0) =
 | Now: (s -> Type0) -> ltl_syntax s
 
 let rec suffixes_of (l:list 'a) : list (list 'a) =
-match l with
-| [] -> []
-| h::tl -> [l] @ (suffixes_of tl)
+  match l with
+  | [] -> []
+  | h::tl -> l :: suffixes_of tl
 
-/// Give the denotation of an ltl formula [form] given a finite trace [tr: list s]
+/// Does a finite trace [tr: list s] satisfy an ltl formula [form]
 let rec ltl_denote (#s: Type0)(form: ltl_syntax s)(tr: list s): Type0 =
   match form with
   | Now p -> ~(tr == []) /\ p (hd tr)
-  //| Eventually p -> exists (i: nat). i <= length tr /\ ltl_denote p (snd (splitAt i tr))
-  //| Always p -> forall (i: nat). i <= length tr ==> ltl_denote p (snd (splitAt i tr))
   | Eventually p -> exists (tl:list s). tl `memP` suffixes_of tr /\ ltl_denote p tl
   | Always p -> forall (tl:list s). tl `memP` suffixes_of tr ==> ltl_denote p tl
   | And p q -> ltl_denote p tr /\ ltl_denote q tr
@@ -396,18 +394,18 @@ let rec ltl_denote (#s: Type0)(form: ltl_syntax s)(tr: list s): Type0 =
 type qltl_formula s = quant * ltl_syntax s
 
 /// Satisfiability of a QLTL formula over sets of finite traces [trs] (non-empty)
-// TODO: why is rec making a difference later?
-let rec qltl_denote (#t: Type0) (form: qltl_formula t) (trs: list (list t)): Type0 =
+// TODO: why is [rec] making a difference later?
+let rec qltl_denote (#t: Type0) (form: qltl_formula t) (trs: list (list t) {Cons? trs}): Type0 =
   match form with
   | (Forall, p) -> forall t. t `memP` trs ==> ltl_denote p t
   | (Exists, p) -> exists t. t `memP` trs /\ ltl_denote p t
-  // match form, trs with
-  //| (Forall, p), [] -> True
-  //| (Forall, p), t::tl -> ltl_denote p t /\ qltl_denote form tl
-  //| (Exists, p), [] -> False
-  //| (Exists, p), t::trs' -> ltl_denote p t \/ qltl_denote form trs'
 
-// Some assertions, SMT is getting stuck on quantifiers I think
+// Some assertions
 let _ = assert(qltl_denote (Forall, Eventually (Now (fun n -> n % 2 == 1))) [[0; 1]; [3]])
 let _ = assert(qltl_denote (Forall, Always (Now (fun n -> n % 2 == 1))) [[1]; [3]]) 
-let _ = assert(qltl_denote (Exists, Always (Now (fun n -> n % 2 == 1))) [[4]; [6]; [2]; [1]; [2]])
+
+let _ = assert(qltl_denote (Exists, Always (Now (fun n -> n % 2 == 1))) [[4]; [6]; [2]; [1]; [2]]) 
+  by (compute(); dump "H")
+
+// Should fail
+let _ = assert(qltl_denote (Forall, Eventually (Now (fun n -> n % 2 == 0))) [[1;3]; [1]]) by (tadmit ())
